Before remove op from value

new_proof/Atom.v
@@ -6,7 +6,7 @@ Definition aset := stringset.
 
 Class Stale {D} A := stale : A -> D.
 
-Definition fv_of_set (s: aset) := fresh_string_of_set "x" s.
+Definition fv_of_set (s: aset): atom := fresh_string_of_set "x" s.
 Lemma fv_of_set_fresh (s: aset) : (fv_of_set s) ∉ s.
 Proof.
   apply fresh_string_of_set_fresh.
