new_proof/BasicTypingProp.v
@@ -92,6 +92,8 @@ Qed.
 (* subst *)
 
 Ltac basic_typing_solver1 :=
+  step_regular_simp;
+  basic_typing_regular_simp;
   listctx_set_simpl;
   (match goal with
    | [H: ?Γ1 ⊢t ?u ⋮v ?T |- (?Γ1 ++ ?Γ2) ⊢t ?u ⋮v ?T ] =>
@@ -101,7 +103,7 @@ Ltac basic_typing_solver1 :=
    | [H: _ ⊢t ?u ⋮v _ |- lc (tvalue ?u)] => apply basic_typing_regular_value in H; destruct H; auto
    | [H: _ ⊢t ?u ⋮t _ |- lc ?u] => apply basic_typing_regular_tm in H; destruct H; auto
    end || lc_solver ||
-       listctx_set_solver).
+     listctx_set_solver || eauto).
 
 Lemma basic_typing_subst_value_aux: forall Γ (v: value) T,
     Γ ⊢t v ⋮v T ->
@@ -114,11 +116,12 @@ Proof.
                 Γ = Γ1 ++ [(z, U)] ++ Γ3 -> Γ1 ⊢t u ⋮v U -> (Γ1 ++ Γ3) ⊢t {z := u}t e ⋮t T)
         ); simpl; intros; subst; listctx_set_simpl;
     try (var_dec_solver; basic_typing_solver1);
-    try (econstructor; listctx_set_solver).
+    try (econstructor; listctx_set_solver1).
   - econstructor. instantiate_atom_listctx.
     rewrite <- subst_open_var_tm; basic_typing_solver1.
   - econstructor. instantiate_atom_listctx.
     rewrite <- subst_open_var_tm; basic_typing_solver1.
+  - econstructor; basic_typing_solver1.
   - econstructor. instantiate (1:= T1). basic_typing_solver1.
     instantiate_atom_listctx; rewrite <- subst_open_var_tm; basic_typing_solver1.
   - econstructor.
@@ -129,6 +132,7 @@ Proof.
   - econstructor.
     instantiate (1:= Tx). instantiate (1:= T1). basic_typing_solver1. basic_typing_solver1.
     instantiate_atom_listctx; rewrite <- subst_open_var_tm; basic_typing_solver1.
+  - econstructor; basic_typing_solver1.
 Qed.
 
 Lemma basic_typing_subst_tm_aux: forall Γ (v: tm) T,
@@ -147,6 +151,7 @@ Proof.
     rewrite <- subst_open_var_tm; basic_typing_solver1.
   - econstructor. instantiate_atom_listctx.
     rewrite <- subst_open_var_tm; basic_typing_solver1.
+  - econstructor; basic_typing_solver1.
   - econstructor. instantiate (1:= T1). basic_typing_solver1.
     instantiate_atom_listctx; rewrite <- subst_open_var_tm; basic_typing_solver1.
   - econstructor.
@@ -157,6 +162,7 @@ Proof.
   - econstructor.
     instantiate (1:= Tx). instantiate (1:= T1). basic_typing_solver1. basic_typing_solver1.
     instantiate_atom_listctx; rewrite <- subst_open_var_tm; basic_typing_solver1.
+  - econstructor; basic_typing_solver1.
 Qed.
 
 Lemma basic_typing_subst_value: forall Γ1 z u U Γ3 (v: value) T,
@@ -189,13 +195,6 @@ Qed.
 
 (* Lemma basic_typing_subst_value_post *)
 
-Ltac basic_typing_simpl1 :=
-  listctx_set_simpl;
-  repeat match goal with
-  | [H: ?Γ ⊢t (tvalue ?v) ⋮t ?T |- _ ] => inversion H; subst; clear H; auto
-  end.
-
-
 Lemma eval_op_type_safe: forall op c1 c2 c3 (T1 T2 T3: base_ty),
   eval_op op c1 c2 c3 ->
   ty_of_op op = T1 ⤍ T2 ⤍ T3 ->
@@ -225,21 +224,26 @@ Proof.
   eapply eval_op_preservation_aux; eauto.
 Qed.
 
+Ltac basic_typing_simpl1 :=
+  step_regular_simp;
+  basic_typing_regular_simp;
+  listctx_set_simpl;
+  repeat match goal with
+    | [H: ?Γ ⊢t (tvalue ?v) ⋮t ?T |- _ ] => inversion H; subst; clear H; auto
+    end.
+
+
 Ltac basic_typing_solver2 :=
   basic_typing_simpl1;
   try match goal with
-      | [H: ?Γ ⊢t (vbiop _) ⋮v _ ⤍ _ ⤍ ?T |- ?Γ ⊢t (vconst _) ⋮v ?T ] => eapply eval_op_preservation; eauto
-      end;
-  basic_typing_solver1.
-
-Ltac auto_pose_fv a Ha :=
-  let acc := collect_stales tt in pose (fv_of_set acc) as a;
-                                  pose (fv_of_set_fresh acc) as Ha.
+    | [H: ?Γ ⊢t (vbiop _) ⋮v _ ⤍ _ ⤍ ?T |- ?Γ ⊢t (vconst _) ⋮v ?T ] => eapply eval_op_preservation; eauto
+    end;
+  (basic_typing_solver1).
 
 Ltac perservation_aux a Ha Tx :=
   match goal with
   | [H: forall (x:atom), _ -> _ ⊢t ?e ^t^ (vfvar x) ⋮t ?T |- _ ⊢t ?e ^t^ ?v ⋮t ?T ] =>
-      auto_pose_fv a Ha; rewrite <- (subst_intro_tm _ a);
+      auto_pose_fv a; rewrite <- (subst_intro_tm _ a);
       try (eapply basic_typing_subst_tm_pre; try basic_typing_solver2; apply H; basic_typing_solver2);
       try (apply basic_typing_subst_tm_pre with (U := Tx); basic_typing_solver2);
       try basic_typing_solver2
@@ -255,15 +259,14 @@ Proof.
     end; auto.
   - econstructor; auto; instantiate_atom_listctx; auto_apply; listctx_set_solver.
   - perservation_aux a Ha Tx.
-  - perservation_aux a Ha Tx.
+  - perservation_aux a Ha Tx. apply H2; basic_typing_solver2.
   - inversion H; subst; clear H. econstructor. instantiate (1:= Tx).
     + perservation_aux a Ha Tx.
     + instantiate_atom_listctx; auto_apply; listctx_set_solver.
-  - inversion H; subst; clear H. auto_pose_fv a Ha. eapply T_LetApp with (T1:=T1) (Tx:=Tx); auto.
-    + rewrite <- (subst_intro_value _ a).
-      eapply basic_typing_subst_value_pre; try basic_typing_solver2. apply H6; basic_typing_solver2.
-      econstructor; basic_typing_solver2. basic_typing_solver2. basic_typing_solver2.
-    + instantiate_atom_listctx; auto_apply; listctx_set_solver.
+  - inversion H; subst; clear H. auto_pose_fv a. eapply T_LetApp; eauto.
+    + rewrite <- (subst_intro_value _ a);
+        try (eapply basic_typing_subst_value_pre; try (apply H6; basic_typing_solver2); basic_typing_solver2);
+        basic_typing_solver2.
 Qed.
 
 (* multi preservation *)
@@ -280,3 +283,105 @@ Proof.
   intros.
   eapply multi_preservation in H0; eauto. inversion H0; subst; auto.
 Qed.
+
+Ltac op_simpl :=
+  basic_typing_simpl1;
+  repeat match goal with
+  | [H: _ ^t^ _ = terr |- _ ] => apply open_eq_terr in H; subst
+  | [H: tlete terr _ ↪* (tvalue _) |- _ ] => apply tlete_terr_exfalso in H; inversion H
+  | [H: tlete (tvalue _) _ ↪* (tvalue _) |- _ ] => rewrite tlete_value_exists in H; repeat destruct_hyp_conj; auto
+  | [ |- ex (fun v_x => tvalue ?v ↪* tvalue v_x /\ _)] => exists v; split; auto
+  end.
+
+Ltac op_solver :=
+  op_simpl;
+  auto;
+  repeat match goal with
+    | [H: _ ⊢t ?e ⋮t _ |- lc ?e ] => apply basic_typing_regular_tm in H; destruct H; auto
+    (* | [H: basicR _ ?e |- lc ?e ] => apply basicR_typable_empty in H; auto *)
+    (* | [H: basicR _ ?e |- [] ⊢t ?e ⋮t _ ] => apply basicR_typable_empty in H; eauto *)
+    | [H: _ ↪ ?e |- lc ?e] => apply multi_step_regular2 in H; auto
+    | [H: ?Γ ⊢t ?e ⋮t ?T |- (?Γ ++ _) ⊢t ?e ⋮t _] => apply basic_typing_weaken_tm_pre; eauto
+    | [H: ?Γ ⊢t _ ⋮t _ |- ok _ ] => apply basic_typing_regular_tm in H; destruct H
+    end; listctx_set_solver.
+
+Ltac basic_typing_vfavr_solver_slow :=
+  op_simpl;
+  match goal with
+  | [|- _ ∉ _ ] => listctx_set_solver
+  | [|- ok _ ] => op_solver
+  | [|- ctxfind _ _ = Some _ ] => repeat var_dec_solver
+  | [|- [(_, _); (_, _)] ⊢t (vfvar ?x) ⋮v _ ] => constructor; basic_typing_vfavr_solver_slow
+  | [|- [(_, _); (_, _); (_, _)] ⊢t (vfvar ?x) ⋮v _ ] => constructor
+                                                       (* ; basic_typing_vfavr_solver *)
+  | [|- [(_, _)] ⊢t (vfvar ?x) ⋮v _ ] => constructor; basic_typing_vfavr_solver_slow
+  | [|- (_ ++ _) ⊢t (tvalue (vfvar ?x)) ⋮t _] => econstructor; op_simpl
+  | [|- (_ ++ _) ⊢t (vfvar ?x) ⋮v _] =>
+      apply basic_typing_weaken_value_post; eauto; basic_typing_vfavr_solver_slow
+  end.
+
+Lemma ok_cache_l3: forall Γ (x1 x2 x3: atom) (T1 T2 T3: ty),
+  ok Γ ->
+  x1 ∉ stale Γ ->
+  x2 ∉ stale Γ ∪ {[x1]} ->
+  x3 ∉ stale Γ ∪ {[x1; x2]} ->
+  ok (Γ ++ [(x1, T1); (x2, T2); (x3, T3)]).
+Proof.
+  intros. repeat basic_typing_vfavr_solver_slow.
+Qed.
+
+Lemma ok_cache_l2: forall Γ (x1 x2: atom) (T1 T2: ty),
+  ok Γ ->
+  x1 ∉ stale Γ ->
+  x2 ∉ stale Γ ∪ {[x1]} ->
+  ok (Γ ++ [(x1, T1); (x2, T2)]).
+Proof.
+  intros. repeat basic_typing_vfavr_solver_slow.
+Qed.
+
+Lemma vfvar_cache_l33: forall Γ (x1 x2 x3: atom) (T1 T2 T3: ty) e T,
+  Γ ⊢t e ⋮t T ->
+  x1 ∉ stale Γ ->
+  x2 ∉ stale Γ ∪ {[x1]} ->
+  x3 ∉ stale Γ ∪ {[x1; x2]} ->
+  (Γ ++ [(x1, T1); (x2, T2); (x3, T3)]) ⊢t x3 ⋮v T3.
+Proof.
+  intros. repeat basic_typing_vfavr_solver_slow.
+Qed.
+
+Lemma vfvar_cache_l22: forall Γ (x1 x2: atom) (T1 T2: ty) e T,
+  Γ ⊢t e ⋮t T ->
+  x1 ∉ stale Γ ->
+  x2 ∉ stale Γ ∪ {[x1]} ->
+  (Γ ++ [(x1, T1); (x2, T2)]) ⊢t x2 ⋮v T2.
+Proof.
+  intros. repeat basic_typing_vfavr_solver_slow.
+Qed.
+
+Lemma vfvar_cache_l21: forall Γ (x1 x2: atom) (T1 T2: ty) e T,
+  Γ ⊢t e ⋮t T ->
+  x1 ∉ stale Γ ->
+  x2 ∉ stale Γ ∪ {[x1]} ->
+  (Γ ++ [(x1, T1); (x2, T2)]) ⊢t x1 ⋮v T1.
+Proof.
+  intros. repeat basic_typing_vfavr_solver_slow.
+Qed.
+
+Ltac basic_typing_vfavr_solver :=
+  op_simpl;
+  match goal with
+  | [H: ?Γ ⊢t _ ⋮t _ |- (?Γ ++ [(_, _); (_, _); (?x, _)]) ⊢t (vfvar ?x) ⋮v _ ] => eapply vfvar_cache_l33; eauto; listctx_set_solver
+  | [H: ?Γ ⊢t _ ⋮t _ |- (?Γ ++ [(_, _); (?x, _)]) ⊢t (vfvar ?x) ⋮v _ ] => eapply vfvar_cache_l22; eauto; listctx_set_solver
+  | [H: ?Γ ⊢t _ ⋮t _ |- (?Γ ++ [(?x, _); (_, _)]) ⊢t (vfvar ?x) ⋮v _ ] => eapply vfvar_cache_l21; eauto; listctx_set_solver
+  | [ |- ok (?Γ ++ [(_, _); (_, _)]) ] => eapply ok_cache_l2; eauto; listctx_set_solver
+  | [ |- ok (?Γ ++ [(_, _); (_, _); (_, _)]) ] => eapply ok_cache_l3; eauto; listctx_set_solver
+  | [|- _ ∉ _ ] => listctx_set_solver
+  | [|- ok _ ] => op_solver
+  | [|- ctxfind _ _ = Some _ ] => repeat var_dec_solver
+  | [|- [(_, _); (_, _)] ⊢t (vfvar ?x) ⋮v _ ] => constructor; basic_typing_vfavr_solver
+  | [|- [(_, _); (_, _); (_, _)] ⊢t (vfvar ?x) ⋮v _ ] => constructor; basic_typing_vfavr_solver
+  | [|- [(_, _)] ⊢t (vfvar ?x) ⋮v _ ] => constructor; basic_typing_vfavr_solver
+  | [|- (_ ++ _) ⊢t (tvalue (vfvar ?x)) ⋮t _] => econstructor; eauto; basic_typing_vfavr_solver
+  | [|- (_ ++ _) ⊢t (vfvar ?x) ⋮v _] =>
+      apply basic_typing_weaken_value_post; eauto; basic_typing_vfavr_solver
+  end.
