new_proof/ErrOperationalSemantics.v
@@ -1,0 +1,261 @@
+From stdpp Require Import mapset.
+From Coq Require Import Logic.ClassicalFacts.
+From Coq Require Import Classical.
+From CT Require Import CoreLang.
+From CT Require Import CoreLangProp.
+From CT Require Import BasicTypingProp.
+
+Import Atom.
+Import CoreLang.
+Import Tactics.
+Import NamelessTactics.
+Import ListCtx.
+Import OperationalSemantics.
+Import BasicTyping.
+Import BasicTypingProp.
+
+Reserved Notation "t1 '⥇' t2" (at level 60).
+
+Inductive err_step : tm -> tm -> Prop :=
+| ErrST_Lete1: forall e1 e1' e,
+    body e ->
+    e1 ⥇ e1' ->
+    (tlete e1 e) ⥇ (tlete e1' e)
+| ErrST_Lete2: forall e,
+    body e -> (tlete terr e) ⥇ terr
+where "t1 '⥇' t2" := (err_step t1 t2).
+
+Definition relation (X : Type) := X -> X -> Prop.
+
+Lemma err_step_regular: forall e1 e2, e1 ⥇ e2 -> lc e1 /\ lc e2.
+Proof.
+  intros.
+  induction H; split; repeat destruct_hyp_conj; auto; destruct H; econstructor; eauto.
+Qed.
+
+Lemma err_step_regular1: forall e1 e2, e1 ⥇ e2 -> lc e1.
+Proof.
+  intros. apply err_step_regular in H. destruct H; auto.
+Qed.
+
+Lemma err_step_regular2: forall e1 e2, e1 ⥇ e2 -> lc e2.
+Proof.
+  intros. apply err_step_regular in H. destruct H; auto.
+Qed.
+
+Global Hint Resolve err_step_regular1: core.
+Global Hint Resolve err_step_regular2: core.
+
+Inductive multierrstep : relation tm :=
+| multierr_step_refl : forall (x : tm),
+    lc x ->
+    multierrstep x x
+| multierr_step_step : forall (x y z : tm),
+    err_step x y ->
+    multierrstep y z ->
+    multierrstep x z.
+
+Global Hint Constructors multierrstep : core.
+
+Theorem multierr_step_R : forall (x y : tm),
+    err_step x y -> multierrstep x y.
+Proof.
+  intros x y H.
+  apply multierr_step_step with y. apply H. apply multierr_step_refl; eauto.
+Qed.
+
+Theorem multierr_step_trans :
+  forall (x y z : tm),
+      multierrstep x y  ->
+      multierrstep y z ->
+      multierrstep x z.
+Proof.
+  intros x y z G H.
+  induction G.
+    - (* multierr_step_refl *) assumption.
+    - (* multierr_step_step *)
+      apply multierr_step_step with y. assumption.
+      apply IHG. assumption.
+Qed.
+
+Definition normal_form (t : tm) : Prop :=
+  ~ exists t', t ⥇ t'.
+
+Definition deterministic {tm : Type} (R : relation tm) :=
+  forall x y1 y2 : tm, R x y1 -> R x y2 -> y1 = y2.
+
+Notation "t1 '⥇*' t2" := (multierrstep t1 t2) (at level 40).
+
+Lemma multi_err_step_regular: forall e1 e2, e1 ⥇* e2 -> lc e1 /\ lc e2.
+Proof.
+  intros.
+  induction H; auto. destruct IHmultierrstep. split; auto. eapply err_step_regular1; eauto.
+Qed.
+
+Lemma multi_err_step_regular1: forall e1 e2, e1 ⥇* e2 -> lc e1.
+Proof.
+  intros. apply multi_err_step_regular in H. destruct H; auto.
+Qed.
+
+Lemma multi_err_step_regular2: forall e1 e2, e1 ⥇* e2 -> lc e2.
+Proof.
+  intros. apply multi_err_step_regular in H. destruct H; auto.
+Qed.
+
+Ltac err_step_regular_simp :=
+  repeat match goal with
+    | [H: _ ⥇ _ |- lc _] => apply err_step_regular in H; destruct H; auto
+    | [H: _ ⥇ _ |- body _] => apply err_step_regular in H; destruct H; auto
+    | [H: _ ⥇* _ |- lc _] => apply multi_err_step_regular in H; destruct H; auto
+    | [H: _ ⥇* _ |- body _] => apply multi_err_step_regular in H; destruct H; auto
+    end.
+
+Lemma err_preservation: forall Γ T (e e': tm), e ⥇ e' -> Γ ⊢t e ⋮t T -> Γ ⊢t e' ⋮t T.
+Proof.
+  intros. generalize dependent e'.
+  induction H0; intros; auto;
+    match goal with
+    | [H: _ ⥇ _ |- _ ] => inversion H; subst
+    end; auto.
+  - econstructor; auto; instantiate_atom_listctx; auto_apply; listctx_set_solver.
+  - constructor. basic_typing_solver2.
+Qed.
+
+Lemma multi_err_preservation: forall Γ T (e e': tm), e ⥇* e' -> Γ ⊢t e ⋮t T -> Γ ⊢t e' ⋮t T.
+Proof.
+  intros.
+  induction H; auto.
+  - apply IHmultierrstep. eapply err_preservation; eauto.
+Qed.
+
+Ltac destruct_hyp_disj :=
+  repeat match goal with
+    | [H: _ \/ _ |- _ ] => destruct H
+    end.
+
+Ltac progress_solver a :=
+  (* repeat match goal with *)
+  (*   (* | [H: forall x, _ -> (_ \/ _) \/ (_ \/ _) |- _ ] => auto_pose_fv a; repeat specialize_with a *) *)
+  (*   | [H: _ \/ _ |- _ ] => destruct H *)
+  (* end; *)
+  match goal with
+  | [H: ∃ e', _ ⥇ e' |- _ ] => right; left; destruct H
+  | [H: exists e', _ ↪ e' |- _] => left; left; destruct H
+  | [H: exists v, _ = tvalue v |- _] => left; left; destruct H; subst
+  | [H: _ = terr |- _ ] => subst; right; left; eexists; eapply ErrST_Lete2
+  | [ |- body _ ] => auto_exists_L; intro a; intros; repeat specialize_with a; basic_typing_solver2
+  | [|- lc _] => basic_typing_solver2
+  end.
+
+Lemma empty_basic_typing_base_const_exists: forall (v: value) (B: base_ty), [] ⊢t v ⋮v B -> (exists (c: constant), v = c).
+Proof.
+  intros. inversion H; subst.
+  - exists c; auto.
+  - inversion H1.
+Qed.
+
+Lemma empty_basic_typing_bool_value_exists: forall (v: value), [] ⊢t v ⋮v TBool -> v = true \/ v = false.
+Proof.
+  intros. inversion H; subst.
+  - destruct c; inversion H0. destruct b; inversion H0. left; auto. right; auto.
+  - inversion H1.
+Qed.
+
+Lemma empty_basic_typing_int_value_exists: forall (v: value), [] ⊢t v ⋮v TNat -> (exists (i: nat), v = i).
+Proof.
+  intros. inversion H; subst.
+  - destruct c; inversion H0. exists n; auto.
+  - inversion H1.
+Qed.
+
+Lemma empty_basic_typing_eval_op_result_exists: forall (op:biop) (v1 v2: value) (T1 T2 Tx: base_ty),
+    [] ⊢t op ⋮v T1 ⤍ T2 ⤍ Tx -> [] ⊢t v2 ⋮v T2 -> [] ⊢t v1 ⋮v T1 ->
+    exists (c1 c2 c3: constant), v1 = c1 /\ v2 = c2 /\ eval_op op c1 c2 c3 /\ [] ⊢t c3 ⋮v Tx.
+Proof.
+  intros.
+  inversion H; subst.
+  assert (exists (c1: constant), v1 = c1) as Htmp. eapply empty_basic_typing_base_const_exists; eauto. destruct Htmp; subst.
+  assert (exists (c2: constant), v2 = c2) as Htmp. eapply empty_basic_typing_base_const_exists; eauto. destruct Htmp; subst.
+  destruct op;
+    simpl in H0; apply empty_basic_typing_int_value_exists in H0; destruct H0; subst;
+    simpl in H1; apply empty_basic_typing_int_value_exists in H1; destruct H1; subst.
+  - exists x2, x1, (x2 + x1). repeat split; auto. econstructor; auto.
+  - exists x2, x1, (Nat.eqb x2 x1). repeat split; auto. econstructor; auto.
+  - exists x2, x1, (Nat.ltb x2 x1). repeat split; auto. econstructor; auto.
+  - exists x2, x1, 0. repeat split; auto. econstructor; auto.
+Qed.
+
+Lemma empty_basic_typing_arrow_value_lam_exists: forall (v: value) T1 T2, [] ⊢t v ⋮v T1 ⤍ T2 ->
+                                                                     (exists (op:biop), v = op) \/
+                                                                     (exists e, v = vlam T1 e) \/ (exists e, v = vfix (T1 ⤍ T2) (vlam T1 e)).
+Proof.
+  intros. inversion H; subst.
+  - left. exists op; auto.
+  - inversion H1.
+  - right; left. exists e; auto.
+  - right; right; exists e; auto.
+Qed.
+
+Lemma progress: forall e T, [] ⊢t e ⋮t T -> ((exists e', e ↪ e') \/ (exists v, e = tvalue v)) \/ ((exists e', e ⥇ e') \/ (e = terr)).
+Proof.
+  intros e T H. remember [] as Γ; induction H; intros; subst;
+    repeat match goal with
+      | [H: [] = [] -> _ |- _ ] =>
+          assert (([]: listctx ty) = []) as Htmp by auto; specialize (H Htmp); try clear Htmp
+      end.
+  - right; right; auto.
+  - left; right; exists v; auto.
+  - destruct_hyp_disj.
+    + repeat progress_solver a. eexists; econstructor; eauto; progress_solver a.
+    + progress_solver a; exists (e2 ^t^ x); constructor; auto; progress_solver a.
+    + progress_solver a; eexists; econstructor; eauto; progress_solver a.
+    + repeat progress_solver a.
+  - left; left. eapply empty_basic_typing_eval_op_result_exists in H1; eauto.
+    destruct H1 as (c1 & c2 & c3 & Hc). repeat destruct_hyp_conj; subst.
+    exists (e ^t^ c3). econstructor; eauto; progress_solver a.
+  - left; left. eapply empty_basic_typing_arrow_value_lam_exists in H.
+    destruct_hyp_disj; destruct 
+    + 
+    destruct H.
+  - apply empty_basic_typing_bool_value_exists in H.
+    destruct H; subst; try clear H;
+    left; left; eexists; econstructor; eauto; progress_solver a.
+  
+    + clear IHtm_has_type2. left; left; eexists; econstructor; eauto; progress_solver a.
+    + 
+
+      left; left; eexists; econstructor; eauto; progress_solver a.
+      left; left; eexists; econstructor; eauto; progress_solver a.
+      subst.
+
+
+
+
+    match goal with
+    | [H: [] = [] -> _ |- _ ] =>
+        assert (([]: listctx ty) = []) as Htmp by auto; specialize (H Htmp); try clear Htmp
+    end. left; left. admit.
+  - left; left. admit.
+  - admit.
+  - admit.
+  - admit.
+  - admit.
+  - admit.
+  
+
+    progress_solver a.
+    eexists; econstructor; eauto. progress_solver a.
+  - progress_solver a.
+    exists (e2 ^t^ x); constructor; auto; progress_solver a.
+  - progress_solver a.
+    eexists; econstructor; eauto; progress_solver a.
+  -  match goal with
+     
+     end. 
+  - auto_pose_fv a; repeat specialize_with a.
+    repeat match goal with
+    | [H: _ \/ _ |- _ ] => destruct H
+    end.
+    progress_solver a.
+
+    eexists; econstructor; eauto. auto_exists_L. intros. repeat specialize_with x0. basic_typing_solver2.
