new_proof/ErrOperationalSemanticsProp.v
@@ -1,0 +1,36 @@
+From stdpp Require Import mapset.
+From Coq Require Import Logic.ClassicalFacts.
+From Coq Require Import Classical.
+From CT Require Import CoreLang.
+From CT Require Import CoreLangProp.
+From CT Require Import BasicTypingProp.
+
+Import Atom.
+Import CoreLang.
+Import Tactics.
+Import NamelessTactics.
+Import ListCtx.
+Import OperationalSemantics.
+Import BasicTyping.
+Import BasicTypingProp.
+
+(* err perservation *)
+Lemma err_preservation: forall Γ T (e e': tm), e ⥇ e' -> Γ ⊢t e ⋮t T -> Γ ⊢t e' ⋮t T.
+Proof.
+  intros. generalize dependent e'.
+  induction H0; intros; auto;
+    match goal with
+    | [H: _ ⥇ _ |- _ ] => inversion H; subst
+    end; auto.
+  - econstructor; auto; instantiate_atom_listctx; auto_apply; listctx_set_solver.
+  - constructor. basic_typing_solver2.
+Qed.
+
+Lemma multi_err_preservation: forall Γ T (e e': tm), e ⥇* e' -> Γ ⊢t e ⋮t T -> Γ ⊢t e' ⋮t T.
+Proof.
+  intros.
+  induction H; auto.
+  - apply IHmultierrstep. eapply err_preservation; eauto.
+Qed.
+
+Lemma progress: forall Γ e T, Γ ⊢t e ⋮t T -> ((exists e', e ↪ e') \/ (exists v', e = tvalue v)) \/ ((exists e', e ⥇ e') \/ (e = terr)).
